policy_proof/coq/query.v
@@ -20,6 +20,8 @@ Inductive trans_func (ℓ1 ℓ2: Policy.policy): Set :=
   | trans_func_with_label: ∀ bt, transform_func bt → trans_func ℓ1 ℓ2
 .
 
+Definition trans_func_denote ℓ1 ℓ2 (f: trans_func ℓ1 ℓ2) : basic_type -> basic_type. Admitted.
+
 Fixpoint schema_to_anf (s: schema): list nat :=
   match s with
     | nil => nil
@@ -157,18 +159,22 @@ Inductive step_cell: ∀ ℓ1 ℓ2, trans_func ℓ1 ℓ2 → config → config �
           ⟨ s Γ β e ⟩ >[ f ]> ⟨ s Γ β e ⟩
   (* This transition is ok. *)
   | E_CTransOk:
-      ∀ ℓ1 ℓ2 ℓcur ℓdisc s Γ β e (f: trans_func ℓ1 ℓ2) (non_empty: List.length e > 0)
-        tl (tl_non_empty: List.length tl > 0) t c_idx,
+      ∀ ℓ1 ℓ2 ℓcur ℓdisc s Γ Γ' β e e' (f: trans_func ℓ1 ℓ2) (non_empty: List.length e > 0)
+        tl tl' (tl_non_empty: List.length tl > 0) t t' c c' c_idx (idx_bound: c_idx < List.length s),
           (* tl => A list of tuples. *)
           tl = (env_slice_get_tuples (get_env_slice s e non_empty)) →
           (* t => The first tuple. *)
           t = hd_ok tl tl_non_empty →
           (* we now get the label encodings. *)
           Some (ℓcur, Some ℓdisc) = Policy.label_lookup c_idx Γ →
-          (* we now get the label encodings. *)
-          ℓcur ⊑ ℓ1 →
-          (* TODO: Update the policy encoding as well as the environment. *)
-          ⟨ s Γ β e ⟩ >[ f ]> ⟨ s Γ β e ⟩
+          (* udpate the policy environment. *)
+          ℓcur ⊑ ℓ1 → Γ' = Policy.update_label c_idx Γ (ℓ2, Some ℓdisc) →
+          (* TODO: Update the tuple. *)
+          tl' = set_nth tl 0 →
+          c = Tuple.nth _ c_idx idx_bound → c' = (trans_func_denote _ _ f) c →
+          t' = Tuple.set_nth_type_match _ c_idx c' idx_bound t →
+          (* update the environment. *)
+          ⟨ s Γ β e ⟩ >[ f ]> ⟨ s Γ' β e' ⟩
 where "c1 '>[' f ']>' c2" := (step_cell _ _ f c1 c2).
 
 (* 
